Fix the env compute problem in an ad-hoc way; and other related fixes

theories/clang/lang.v
@@ -1,200 +1,16 @@
 (** Language definition **)
 
+From iris_os.lib Require Export smap prelude.
 From iris.algebra Require Export gmap.
-Require Export memory.
-From iris_os.lib Require Export Integers.
+From iris_os.clang Require Export memory types.
+
 Open Scope Z_scope.
 
-Definition ident := Z.
-
-Inductive type : Set :=
-| Tnull
-| Tvoid
-| Tint8
-| Tint32
-| Tptr (t: type)
-| Tprod (t1 t2: type).
-
-(* High-level value *)
-Inductive val : Set :=
-| Vvoid
-| Vnull
-| Vint8 (i: int8)
-| Vint32 (i: int32)
-| Vptr (p: addr)
-| Vpair (v1 v2: val).
-
-Fixpoint type_infer_v (v: val) : type :=
-  match v with
-    | Vnull => Tnull
-    | Vvoid => Tvoid
-    | Vint8 _ => Tint8
-    | Vint32 _ => Tint32
-    | Vptr _ => Tptr Tvoid (* XXX *)
-    | Vpair v1 v2 => Tprod (type_infer_v v1) (type_infer_v v2)
-  end.
-
-Inductive typeof: val → type → Prop :=
-| typeof_null: typeof Vnull Tnull
-| typeof_void: typeof Vvoid Tvoid
-| typeof_int8: ∀ i, typeof (Vint8 i) Tint8
-| typeof_int32: ∀ i, typeof (Vint32 i) Tint32
-| typeof_prod:
-    ∀ v1 v2 t1 t2,
-      typeof v1 t1 → typeof v2 t2 → typeof (Vpair v1 v2) (Tprod t1 t2)
-| typeof_null_ptr: ∀ t, typeof Vnull (Tptr t)
-| typeof_ptr: ∀ l t, typeof (Vptr l) (Tptr t).
-
-Lemma null_typeof v: typeof v Tnull → v = Vnull. Proof. induction v; inversion 1=>//. Qed.
-Lemma void_typeof v: typeof v Tvoid → v = Vvoid. Proof. induction v; inversion 1=>//. Qed.
-Lemma int8_typeof v: typeof v Tint8 → (∃ i, v = Vint8 i). Proof. induction v; inversion 1=>//. eauto. Qed.
-Lemma int32_typeof v: typeof v Tint32 → (∃ i, v = Vint32 i). Proof. induction v; inversion 1=>//. eauto. Qed.
-
-Lemma typeof_any_ptr l t1 t2:
-  typeof l (Tptr t1) → typeof l (Tptr t2).
-Proof. induction l; inversion 1; subst=>//; constructor. Qed.
-
-Instance int_eq_dec : EqDecision int.
-Proof. apply Int.eq_dec. Defined.
-
-Instance byte_eq_dec : EqDecision byte.
-Proof. apply Byte.eq_dec. Defined.
-
-Instance val_eq_dec : EqDecision val.
-Proof. solve_decision. Defined.
-
-Definition vtrue := Vint8 (Byte.repr 1).
-Definition vfalse := Vint8 (Byte.repr 0).
-
-Fixpoint sizeof (t : type) : nat :=
-  match t with
-    | Tnull => 4 %nat
-    | Tvoid => 0 % nat
-    | Tint8 => 1 % nat
-    | Tint32 => 4 % nat
-    | Tptr _ => 4 % nat
-    | Tprod t1 t2 => sizeof t1 + sizeof t2
-  end.
-
-Inductive bop:=
+Inductive bop :=
 | oplus
 | ominus
 | oequals
 | oneq.
-
-(* Encoding and decoding for values *)
-Fixpoint encode_int (n: nat) (x: Z): list byte :=
-  match n with
-    | O => nil
-    | S m => Byte.repr x :: encode_int m (x / 256)
-  end.
-
-Fixpoint decode_int (l: list byte): Z :=
-  match l with
-    | nil => 0
-    | b :: l' => Byte.unsigned b + decode_int l' * 256
-  end.
-
-Lemma encode_int_length:
-  forall sz x, length(encode_int sz x) = sz.
-Proof.
-  induction sz; simpl; intros. auto. decEq. auto.
-Qed.
-
-Definition inj_bytes (bl: list byte) : list byteval := List.map BVint8 bl.
-
-Fixpoint proj_bytes (vl: list byteval) : option (list byte) :=
-  match vl with
-    | nil => Some nil
-    | BVint8 b :: vl' =>
-      match proj_bytes vl' with None => None | Some bl => Some (b :: bl) end
-    | _ => None
-  end.
-
-Lemma length_inj_bytes:
-  forall bl, length (inj_bytes bl) = length bl.
-Proof.
-  intros. apply List.map_length.
-Qed.
-
-Lemma proj_inj_bytes:
-  forall bl, proj_bytes (inj_bytes bl) = Some bl.
-Proof.
-  induction bl; simpl. auto. rewrite IHbl. auto.
-Qed.
-
-Lemma inj_proj_bytes:
-  forall cl bl, proj_bytes cl = Some bl -> cl = inj_bytes bl.
-Proof.
-  induction cl; simpl; intros.
-  inv H; auto.
-  destruct a; try congruence. destruct (proj_bytes cl); inv H.
-  simpl. decEq. auto.
-Qed.
-
-Fixpoint inj_pointer (n: nat) (p: addr): list byteval :=
-  match n with
-    | O => nil
-    | S n => BVaddr p n :: inj_pointer n p
-  end.
-
-Fixpoint check_pointer (n: nat) (p: addr) (vl: list byteval) : bool :=
-  match n, vl with
-    | O, nil => true
-    | S m, BVaddr p' m' :: vl' =>
-      bool_decide (p = p') && beq_nat m m' && check_pointer m p vl'
-    | _, _ => false
-  end.
-
-Definition proj_pointer (vl: list byteval) : option val :=
-  match vl with
-    | BVaddr p n :: vl' =>
-      if check_pointer 4%nat p vl then Some (Vptr p) else None
-    | _ => None
-  end.
-
-Fixpoint encode_val (v: val) : list byteval :=
-  match v with
-    | Vint32 n => inj_bytes (encode_int 4%nat (Int.unsigned n))
-    | Vint8 n => inj_bytes (encode_int 1%nat (Byte.unsigned n))
-    | Vptr p => inj_pointer 4%nat p
-    | Vnull => list_repeat 4 BVnull
-    | Vpair v1 v2 => encode_val v1 ++ encode_val v2
-    | _ => list_repeat (sizeof (type_infer_v v)) BVundef
-  end.
-
-Fixpoint decode_val (t: type) (vl: list byteval) : option val :=
-  match t with
-    | Tprod t1 t2 =>
-      (match decode_val t1 (take (sizeof t1) vl),
-             decode_val t2 (drop (sizeof t1) vl) with
-         | Some v1, Some v2 => Some (Vpair v1 v2)
-         | _, _ => None
-       end)
-    | _ =>
-      (match proj_bytes vl with
-         | Some bl =>
-           match t with
-             | Tint8  => Some (Vint32 (Int.zero_ext 8 (Int.repr (decode_int bl))))
-             | Tint32 => Some (Vint32 (Int.repr (decode_int bl)))
-             | _ => None
-           end
-         | None =>
-           match vl with
-             | BVnull :: BVnull ::BVnull :: BVnull :: nil =>
-               match t with
-                 | Tnull => Some Vnull
-                 | Tptr _ => Some Vnull
-                 | _ => None
-               end
-             | _ =>
-               match t with
-                 | Tptr _ => proj_pointer vl
-                 | _ => None
-               end
-           end
-       end)
-  end.
 
 Inductive expr :=
 | Evalue (v: val)
@@ -262,12 +78,12 @@ Definition context : Type := (exprctx * stmtsctx).
 Inductive cureval :=
 | curs (s: stmts) | cure (e: expr).
 
-Definition env : Type := gmap ident (type * addr).
+Definition env : Type := smap (type * addr).
 
 Fixpoint type_infer (ev: env) (e: expr) : option type :=
   match e with
     | Evalue v => Some (type_infer_v v)
-    | Evar x => p ← ev !! x; Some (p.1)
+    | Evar x => p ← sget x ev; Some (p.1)
     | Ebinop _ e1 _ => type_infer ev e1 (* FIXME *)
     | Ederef e' =>
       (match type_infer ev e' with
@@ -288,8 +104,6 @@ Fixpoint type_infer (ev: env) (e: expr) : option type :=
        end)
     | Ecast _ t => Some t (* FIXME *)
   end.
-
-Definition code : Type := (cureval * context * list context).
 
 Definition fill_expr (e : expr) (Ke : exprctx) : expr :=
   match Ke with
@@ -466,18 +280,6 @@ Lemma reducible_not_ret_val c σ: reducible c σ → to_ret_val c = None.
 Admitted.
 
 Instance state_inhabited: Inhabited state := populate ∅.
-
-Lemma size_of_encode_val v:
-  length (encode_val v) = sizeof (type_infer_v v).
-Proof. induction v=>//. simpl. rewrite app_length. omega. Qed.
-
-Lemma typeof_preserves_size v t:
-  typeof v t → sizeof t = length (encode_val v).
-Admitted.
-
-Lemma type_infer_preserves_size v:
-  sizeof (type_infer_v v) = length (encode_val v).
-Admitted.
 
 Inductive assign_type_compatible : type → type → Prop :=
 | assign_id: ∀ t, assign_type_compatible t t
