theories/clang/lib/list.v
@@ -8,13 +8,13 @@ Section proof.
 
   (* de brujin with autosubst? *)
   Definition tcell (telem: type): type := Tprod telem (Tptr Tvoid).
-  Definition tlist (telem: type): type := Tptr (tcell telem).
+  (* Definition tlist (telem: type): type := Tptr (tcell telem). *)
 
   Fixpoint isList (l: val) (xs: list val) (t: type) :=
     match xs with
       | [] => (⌜ l = null ⌝)%I
       | x::xs' => (∃ p l',
-                     ⌜ l = Vptr p ∧ typeof x t ∧ typeof l' (tlist t) ⌝ ∗
+                     ⌜ l = Vptr p ∧ typeof x t ∧ typeof l' (Tptr (tcell t)) ⌝ ∗
                      p ↦ Vpair x l' @ tcell t ∗ isList l' xs' t)%I
     end.
 
@@ -29,39 +29,43 @@ Section proof.
   Qed.
   
   Parameter py pt px: addr.
-  Parameter x: ident.
+  Definition x: ident := 1.
+  Definition y: ident := 2.
+  Definition t: ident := 3.
 
   Definition rev_list (telem: type) : stmts :=
     while [ x != null ] ( x != null ) <{
-      pt <- snd (!x) ;;
-      snd (!x) <- !py ;;
-      py <- x ;;
-      x <- !pt
+      t <- snd (!x) ;;
+      snd (!x) <- y ;;
+      y <- x ;;
+      x <- t
     }>.
-
+  
   Lemma rev_spec Φ Φret body xs:
     ∀ lx ly ys,
-    instantiate_f_body {[ x := (tlist Tint32, px) ]} (rev_list Tint32) = Some body →
-    isList lx xs Tint32 ∗ isList ly ys Tint32 ∗ pt ↦ - @ Tptr Tvoid ∗
-    px ↦ lx @ tlist Tint32 ∗ py ↦ ly @ tlist Tint32 ∗
-    (∀ ly', py ↦ ly' @ tlist Tint32 ∗ isList ly' (rev xs ++ ys) Tint32 -∗ Φ Vvoid)
+      instantiate_f_body
+        [(x, (Tptr (tcell Tint32), px));
+         (y, (Tptr Tvoid, py));
+         (t, (Tptr (tcell Tint32), pt))]
+        (rev_list Tint32) = Some body →
+    isList lx xs Tint32 ∗ isList ly ys Tint32 ∗ pt ↦ - @ Tptr (tcell Tint32) ∗
+    px ↦ lx @ Tptr (tcell Tint32) ∗ py ↦ ly @ Tptr Tvoid ∗
+    (∀ ly', py ↦ ly' @ Tptr Tvoid ∗ isList ly' (rev xs ++ ys) Tint32 -∗ Φ Vvoid)
     ⊢ WP curs body {{ Φ; Φret }}.
   Proof.
     induction xs as [|x xs' IHxs'];
     unfold_f_inst;
-    destruct (decide (x = x))=>//;
     intros ??? [=]; destruct px; subst.
     - iIntros "(% & Hlr & Ht & Hpx & Hpy & HΦ)".
       subst. wp_load. wp_op.
       iApply wp_while_false.
       iNext. iApply "HΦ". iFrame.
     - iIntros "(Hl & Hlr & Ht & Hpx & Hpy & HΦ)".
-      destruct (decide (proof.x = proof.x))=>//.
       wp_load. iDestruct "Hl" as (p l') "(% & Hp & Hl')".
       destruct H0 as [? [? ?]]. subst.
       wp_op. iApply wp_while_true.
       iNext. repeat (iApply wp_seq).
-      iApply (wp_bind [EKderef; EKsnd] (SKassignl _)). (* TODO: Some bug in tactic *)
+      iApply (wp_bind [EKderef_typed _; EKsnd] (SKassignl _)). (* TODO: Some bug in tactic *)
       iApply wp_load. iFrame. iIntros "!> Hbo".
       simpl. wp_load. wp_bind (Esnd _).
       iApply wp_snd. iNext. iApply wp_value=>//.
@@ -72,18 +76,23 @@ Section proof.
       simpl. iApply (wp_bind [] (SKassignr _)).
       destruct p as [pb po].
       iApply wp_op=>//. simpl.
-      rewrite /offset_by_byte.
+      rewrite /offset_by_byte. 
       replace (Z.to_nat (Byte.intval (Byte.repr 4))) with 4%nat; last done.
       wp_load. iDestruct (isList_ptr with "Hlr") as "%".
-      wp_assign=>//. wp_load. wp_assign. wp_load. wp_assign.
-      iApply (IHxs' l' (Vptr (pb, po)) (x::ys)).
-      { unfold_f_inst. destruct (decide (proof.x = proof.x))=>//. }
-      iFrame.
-      iSplitL "Hp Hlr".
+      wp_assign=>//.
+      wp_load.
+      assert (typeof (Vptr (pb, po)) (Tptr Tvoid)).
+      { constructor. }
+      iApply (wp_assign (Tptr Tvoid) (Tptr Tvoid)).
+      { done. } { constructor. }
+      iFrame. iIntros "!> ?".  
+      wp_load. wp_assign.
+      iApply (IHxs' l' (Vptr (pb, po)) (x::ys)); first by unfold_f_inst.
+      iFrame. iSplitL "Hp Hlr".
       { iExists (pb, po), ly. iFrame.
         iPureIntro. repeat (split; first done). by eapply typeof_any_ptr. }
       iSplitL "Ht"; first eauto.
-      replace (rev xs' ++ x :: ys) with ((rev xs' ++ [x]) ++ ys); first done; last by rewrite -app_assoc.
+      by rewrite -app_assoc.
   Qed.
   
 End proof.
