theories/clang/memory.v
@@ -1,8 +1,14 @@
 (** Definition of the physical memory model **)
 Require Export lib.Coqlib.
 Require Export Integers.
+Require Export iris.base_logic.base_logic.
+
 Open Local Scope Z_scope.
-Require Import iris.base_logic.base_logic.
+
+Class Sizeof C := sizeof: C → nat.
+
+Arguments sizeof _ _ _ /.
+Typeclasses Transparent sizeof.
 
 Definition block : Set := positive.
 Definition offset := nat.
@@ -10,9 +16,127 @@ Definition addr : Set := prod block offset.
 
 Instance addr_eq_dec : EqDecision addr.
 Proof. solve_decision. Defined.
+Instance int_eq_dec : EqDecision int.
+Proof. apply Int.eq_dec. Defined.
+Instance byte_eq_dec : EqDecision byte.
+Proof. apply Byte.eq_dec. Defined.
 
+(* Byte-level value *)
 Inductive byteval : Set :=
 | BVundef
 | BVint8 (i: int8)
 | BVaddr (p: addr) (k: nat)
 | BVnull.
+
+(* High-level value *)
+Inductive val : Set :=
+| Vvoid
+| Vnull
+| Vint8 (i: int8)
+| Vint32 (i: int32)
+| Vptr (p: addr)
+| Vpair (v1 v2: val).
+
+Instance val_eq_dec : EqDecision val.
+Proof. solve_decision. Defined.
+
+Instance sizeof_val: Sizeof val :=
+  fix go v :=
+  match v with
+    | Vnull => 4 %nat
+    | Vvoid => 0 % nat
+    | Vint8 _ => 1 % nat
+    | Vint32 _ => 4 % nat
+    | Vptr _ => 4 % nat
+    | Vpair v1 v2 => (go v1 + go v2)%nat
+  end.
+
+Definition vtrue := Vint8 (Byte.repr 1).
+Definition vfalse := Vint8 (Byte.repr 0).
+
+(** Encoding high-level value to byte-level values **)
+
+Fixpoint encode_int (n: nat) (x: Z): list byte :=
+  match n with
+    | O => nil
+    | S m => Byte.repr x :: encode_int m (x / 256)
+  end.
+
+Fixpoint decode_int (l: list byte): Z :=
+  match l with
+    | nil => 0
+    | b :: l' => Byte.unsigned b + decode_int l' * 256
+  end.
+
+Lemma encode_int_length:
+  forall sz x, length(encode_int sz x) = sz.
+Proof.
+  induction sz; simpl; intros. auto. decEq. auto.
+Qed.
+
+Definition inj_bytes (bl: list byte) : list byteval := List.map BVint8 bl.
+
+Fixpoint proj_bytes (vl: list byteval) : option (list byte) :=
+  match vl with
+    | nil => Some nil
+    | BVint8 b :: vl' =>
+      match proj_bytes vl' with None => None | Some bl => Some (b :: bl) end
+    | _ => None
+  end.
+
+Lemma length_inj_bytes:
+  forall bl, length (inj_bytes bl) = length bl.
+Proof.
+  intros. apply List.map_length.
+Qed.
+
+Lemma proj_inj_bytes:
+  forall bl, proj_bytes (inj_bytes bl) = Some bl.
+Proof.
+  induction bl; simpl. auto. rewrite IHbl. auto.
+Qed.
+
+Lemma inj_proj_bytes:
+  forall cl bl, proj_bytes cl = Some bl -> cl = inj_bytes bl.
+Proof.
+  induction cl; simpl; intros.
+  inv H; auto.
+  destruct a; try congruence. destruct (proj_bytes cl); inv H.
+  simpl. decEq. auto.
+Qed.
+
+Fixpoint inj_pointer (n: nat) (p: addr): list byteval :=
+  match n with
+    | O => nil
+    | S n => BVaddr p n :: inj_pointer n p
+  end.
+
+Fixpoint check_pointer (n: nat) (p: addr) (vl: list byteval) : bool :=
+  match n, vl with
+    | O, nil => true
+    | S m, BVaddr p' m' :: vl' =>
+      bool_decide (p = p') && beq_nat m m' && check_pointer m p vl'
+    | _, _ => false
+  end.
+
+Definition proj_pointer (vl: list byteval) : option val :=
+  match vl with
+    | BVaddr p n :: vl' =>
+      if check_pointer 4%nat p vl then Some (Vptr p) else None
+    | _ => None
+  end.
+
+Fixpoint encode_val (v: val) : list byteval :=
+  match v with
+    | Vint32 n => inj_bytes (encode_int 4%nat (Int.unsigned n))
+    | Vint8 n => inj_bytes (encode_int 1%nat (Byte.unsigned n))
+    | Vptr p => inj_pointer 4%nat p
+    | Vnull => list_repeat 4 BVnull
+    | Vpair v1 v2 => encode_val v1 ++ encode_val v2
+    | _ => list_repeat (sizeof v) BVundef
+  end.
+
+
+Lemma size_of_encode_val v:
+  length (encode_val v) = sizeof v.
+Proof. simpl. induction v=>//. rewrite app_length. simpl. omega. Qed.
