theories/lib/smap.v
@@ -1,69 +1,21 @@
-(* Simple, finite, computable map based on list *)
+(* Simple map structure *)
 
-Require Import iris.prelude.base.
-Require Import iris.prelude.fin_maps.
+Require Import iris_os.lib.prelude.
 
+Definition smap (A: Type) := list (ident * A).
 
-Definition smap K `{EqDecision K} A := list (K * A).
+Definition semp {A: Type} : smap A := nil.
 
-Instance smap_fmap `{EqDecision K} : FMap (smap K) := λ A B f m, map (λ kv, ((kv.1), f (kv.2))) m.
-
-Instance smap_lookup `{EqDecision K} A: Lookup K A (smap K A) :=
-  λ k,
-  fix go m :=
+Fixpoint sget {A} k (m: smap A) : option A :=
   match m with
-    | (k', v')::m' => if decide (k' = k) then Some v' else go m'
+    | cons (k', v') m' => if (Zbool.Zeq_bool k' k) then Some v' else sget k m'
     | _ => None
   end.
 
-Instance smap_empty `{EqDecision K} A: Empty (smap K A) := [].
+Definition sset {A: Type} k (v: A) (m: smap A) : smap A := cons (k, v) m.
 
-Instance smap_partial_alter `{EqDecision K} A: PartialAlter K A (smap K A) :=
-  λ f k,
-  fix go m :=
-    match m with
-      | (k', v')::m' =>
-        if decide (k = k') then
-          (match f (Some v') with
-             | Some v'' => (k', v'') :: m' (* alter *)
-             | None => m' (* delete *)
-           end)
-        else (k', v') :: go m'
-      | _ =>
-        match f None with
-          | Some v => [(k, v)]
-          | None => []
-        end
-    end.
+Definition ssig {A: Type} k v : smap A := cons (k, v) nil.
 
-Instance smap_omap `{EqDecision K} : OMap (smap K) :=
-  λ A B f,
-  fix go m :=
-    match m with
-      | (k, v)::m' =>
-        match f v with
-          | Some v' => (k, v'):: go m'
-          | None => go m'
-        end
-      | _ => []
-    end.
-
-Fixpoint smap_merge_by_keys
-         `{EqDecision K} {A B C} (f: option A → option B → option C)
-         (ks: list K) (ma: smap K A) (mb: smap K B) : smap K C :=
-  match ks with
-    | k::ks' =>
-      match f (ma !! k) (mb !! k) with
-        | Some vc => (k, vc) :: smap_merge_by_keys f ks' ma mb
-        | None => smap_merge_by_keys f ks' ma mb
-      end
-    | _ => []
-  end.
-
-Instance smap_to_list `{EqDecision K} A: FinMapToList K A (smap K A) := id.
-
-Instance smap_merge `{eq: EqDecision K}: Merge (smap K) :=
-  λ A B C f ma mb, smap_merge_by_keys f (nodup eq (ma.*1 ++ mb.*1)) ma mb.
-
-Instance smap_finmap `{EqDecision K} : FinMap K (smap K).
-Admitted. (* ALthough I don't know why I should do it at all *)
+Arguments sget {_} _ _.
+Arguments sset {_} _ _ _.
+Arguments ssig {_} _ _.
