theories/clang/opsem.v
@@ -1,0 +1,5 @@
+(* Operational Semantics for the final machine *)
+
+Require Import iris_os.clang.lang.
+
+Definition code : Type := (cureval * context * list context).
