theories/clang/types.v
@@ -1,0 +1,91 @@
+From iris_os.clang Require Import memory.
+
+Inductive type : Set :=
+| Tnull
+| Tvoid
+| Tint8
+| Tint32
+| Tptr (t: type)
+| Tprod (t1 t2: type).
+
+Fixpoint type_infer_v (v: val) : type :=
+  match v with
+    | Vnull => Tnull
+    | Vvoid => Tvoid
+    | Vint8 _ => Tint8
+    | Vint32 _ => Tint32
+    | Vptr _ => Tptr Tvoid (* XXX *)
+    | Vpair v1 v2 => Tprod (type_infer_v v1) (type_infer_v v2)
+  end.
+
+Inductive typeof: val → type → Prop :=
+| typeof_null: typeof Vnull Tnull
+| typeof_void: typeof Vvoid Tvoid
+| typeof_int8: ∀ i, typeof (Vint8 i) Tint8
+| typeof_int32: ∀ i, typeof (Vint32 i) Tint32
+| typeof_prod:
+    ∀ v1 v2 t1 t2,
+      typeof v1 t1 → typeof v2 t2 → typeof (Vpair v1 v2) (Tprod t1 t2)
+| typeof_null_ptr: ∀ t, typeof Vnull (Tptr t)
+| typeof_ptr: ∀ l t, typeof (Vptr l) (Tptr t).
+
+Lemma null_typeof v: typeof v Tnull → v = Vnull. Proof. induction v; inversion 1=>//. Qed.
+Lemma void_typeof v: typeof v Tvoid → v = Vvoid. Proof. induction v; inversion 1=>//. Qed.
+Lemma int8_typeof v: typeof v Tint8 → (∃ i, v = Vint8 i). Proof. induction v; inversion 1=>//. eauto. Qed.
+Lemma int32_typeof v: typeof v Tint32 → (∃ i, v = Vint32 i). Proof. induction v; inversion 1=>//. eauto. Qed.
+
+Lemma typeof_any_ptr l t1 t2:
+  typeof l (Tptr t1) → typeof l (Tptr t2).
+Proof. induction l; inversion 1; subst=>//; constructor. Qed.
+
+Instance sizeof_type: Sizeof type :=
+  fix go (t : type) : nat :=
+  match t with
+    | Tnull => 4 %nat
+    | Tvoid => 0 % nat
+    | Tint8 => 1 % nat
+    | Tint32 => 4 % nat
+    | Tptr _ => 4 % nat
+    | Tprod t1 t2 => go t1 + go t2
+  end.
+
+Lemma typeof_preserves_size v t:
+  typeof v t → sizeof t = length (encode_val v).
+Admitted.
+
+Lemma type_infer_preserves_size v:
+  sizeof (type_infer_v v) = length (encode_val v).
+Admitted.
+
+(* Fixpoint decode_val (t: type) (vl: list byteval) : option val := *)
+(*   match t with *)
+(*     | Tprod t1 t2 => *)
+(*       (match decode_val t1 (take (sizeof t1) vl), *)
+(*              decode_val t2 (drop (sizeof t1) vl) with *)
+(*          | Some v1, Some v2 => Some (Vpair v1 v2) *)
+(*          | _, _ => None *)
+(*        end) *)
+(*     | _ => *)
+(*       (match proj_bytes vl with *)
+(*          | Some bl => *)
+(*            match t with *)
+(*              | Tint8  => Some (Vint32 (Int.zero_ext 8 (Int.repr (decode_int bl)))) *)
+(*              | Tint32 => Some (Vint32 (Int.repr (decode_int bl))) *)
+(*              | _ => None *)
+(*            end *)
+(*          | None => *)
+(*            match vl with *)
+(*              | BVnull :: BVnull ::BVnull :: BVnull :: nil => *)
+(*                match t with *)
+(*                  | Tnull => Some Vnull *)
+(*                  | Tptr _ => Some Vnull *)
+(*                  | _ => None *)
+(*                end *)
+(*              | _ => *)
+(*                match t with *)
+(*                  | Tptr _ => proj_pointer vl *)
+(*                  | _ => None *)
+(*                end *)
+(*            end *)
+(*        end) *)
+(*   end. *)
