theories/lib/prelude.v
@@ -1,0 +1,7 @@
+(* Re-export of Iris and some general stuff *)
+
+Require Import iris_os.lib.Integers.
+
+Open Scope Z_scope.
+
+Definition ident : Set := BinNums.Z.
